fairness/heap_lang/proofmode_lsi.v
@@ -25,13 +25,12 @@ Ltac wp_expr_simpl := wp_expr_eval simpl.
 
 
 Lemma tac_wp_pure_helper `{EM: ExecutionModel heap_lang M} `{@heapGS Σ _ EM} 
-  `{iLM: LiveModel G iM LSI} `{Countable G}
+  `{Countable G} `{iLM: LiveModel G iM LSI} `{Countable G}
   `{PMPP: @PartialModelPredicatesPre (locale heap_lang) _ _ Σ iM}  
   tid E Einvs K e1 e2
   (fs: gmap (fmrole iM) nat)
   (* fs *)
   φ n Φ :
-(* >>>>>>> origin/pmp_resource *)
   fs ≠ ∅ ->
   PureExec φ n e1 e2 →
   φ →
@@ -87,7 +86,7 @@ Lemma has_fuels_gt_1
 Proof. intros ?. by rewrite has_fuels_gt_n //. Qed.
 
 Lemma tac_wp_pure_helper_2 `{EM: ExecutionModel heap_lang M} `{@heapGS Σ _ EM}
-  `{iLM: LiveModel G iM LSI} `{Countable G}
+  `{Countable G} `{iLM: LiveModel G iM LSI} `{Countable G}
   (* `{!fairnessGS iLM Σ}   *)
   `{PMPP: @PartialModelPredicatesPre (locale heap_lang) _ _ Σ iM}
   tid E Einvs K e1 e2
@@ -159,7 +158,7 @@ Proof.
 Qed.
 
 Lemma tac_wp_pure `{EM: ExecutionModel heap_lang M} `{@heapGS Σ _ EM}
-  `{iLM: LiveModel G iM LSI} `{Countable G}
+  `{Countable G} `{iLM: LiveModel G iM LSI} `{Countable G}
   (* `{!fairnessGS iLM Σ}   *)
   `{PMPP: @PartialModelPredicatesPre (locale heap_lang) _ _ Σ iM}
   Δ Δ'other tid E Einvs i K e1 e2 φ n Φ
@@ -360,7 +359,7 @@ Implicit Types Δ : envs (uPredI (iResUR Σ)).
 Implicit Types v : val.
 Implicit Types tid : locale heap_lang.
 
-Context `{iLM: LiveModel G iM LSI} `{Countable G}.
+Context  `{Countable G} `{iLM: LiveModel G iM LSI}.
 Context `{!fairnessGS iLM Σ}. 
 (* Context `{PMP: PartialModelPredicates heap_lang (M := M) (iM := iM) (LM := LM) (iLM := iLM)}.  *)
 Context `{PMPP: @PartialModelPredicatesPre (locale heap_lang) _ _ Σ iM}. 
